case_study/RiscvPmp/BlockVer/Verifier.v
@@ -36,7 +36,7 @@ From Equations Require Import
      Equations.
 From Katamaran Require Import
      Iris.Instance
-     Iris.Model
+     Iris.Base
      Notations
      Semantics
      Bitvector
