case_study/RiscvPmp/IrisInstanceBinary.v
@@ -29,6 +29,8 @@
 From Katamaran Require Import
      Base
      Bitvector
+     Iris.BinaryWeakestPre
+     Iris.BinaryAdequacy
      Iris.BinaryInstance
      trace
      Syntax.Predicates
@@ -46,7 +48,7 @@ Module ns := stdpp.namespaces.
 Set Implicit Arguments.
 Import bv.notations.
 
-Module RiscvPmpIrisAdeqParams2 <: IrisAdeqParameters2 RiscvPmpBase RiscvPmpIrisBase2 RiscvPmpProgram RiscvPmpSemantics RiscvPmpIrisBase2.
+Module RiscvPmpIrisAdeqParams2 <: IrisAdeqParameters2 RiscvPmpBase RiscvPmpProgram RiscvPmpSemantics RiscvPmpIrisBase2 RiscvPmpIrisBase2 RiscvPmpIrisBase2.
 
   Import RiscvPmpIrisAdeqParameters.
   Import RiscvPmpIrisBase2.
@@ -349,6 +351,9 @@ Module RiscvPmpIrisInstance2 <:
       iApply interp_addr_access_byte_inj.
     Qed.
   End RiscVPmpIrisInstanceProofs.
+
+  Include IrisBinaryWP RiscvPmpBase RiscvPmpSignature RiscvPmpProgram
+    RiscvPmpSemantics RiscvPmpIrisBase2.
 
   Include IrisSignatureRules2 RiscvPmpBase RiscvPmpSignature RiscvPmpProgram
     RiscvPmpSemantics RiscvPmpIrisBase2.
