theories/Iris/BinaryWeakestPre.v
@@ -1,0 +1,621 @@
+(******************************************************************************)
+(* Copyright (c) 2020 Dominique Devriese, Sander Huyghebaert, Steven Keuchel  *)
+(* All rights reserved.                                                       *)
+(*                                                                            *)
+(* Redistribution and use in source and binary forms, with or without         *)
+(* modification, are permitted provided that the following conditions are     *)
+(* met:                                                                       *)
+(*                                                                            *)
+(* 1. Redistributions of source code must retain the above copyright notice,  *)
+(*    this list of conditions and the following disclaimer.                   *)
+(*                                                                            *)
+(* 2. Redistributions in binary form must reproduce the above copyright       *)
+(*    notice, this list of conditions and the following disclaimer in the     *)
+(*    documentation and/or other materials provided with the distribution.    *)
+(*                                                                            *)
+(* THIS SOFTWARE IS PROVIDED BY THE COPYRIGHT HOLDERS AND CONTRIBUTORS        *)
+(* "AS IS" AND ANY EXPRESS OR IMPLIED WARRANTIES, INCLUDING, BUT NOT LIMITED  *)
+(* TO, THE IMPLIED WARRANTIES OF MERCHANTABILITY AND FITNESS FOR A PARTICULAR *)
+(* PURPOSE ARE DISCLAIMED. IN NO EVENT SHALL THE COPYRIGHT HOLDER OR          *)
+(* CONTRIBUTORS BE LIABLE FOR ANY DIRECT, INDIRECT, INCIDENTAL, SPECIAL,      *)
+(* EXEMPLARY, OR CONSEQUENTIAL DAMAGES (INCLUDING, BUT NOT LIMITED TO,        *)
+(* PROCUREMENT OF SUBSTITUTE GOODS OR SERVICES; LOSS OF USE, DATA, OR         *)
+(* PROFITS; OR BUSINESS INTERRUPTION) HOWEVER CAUSED AND ON ANY THEORY OF     *)
+(* LIABILITY, WHETHER IN CONTRACT, STRICT LIABILITY, OR TORT (INCLUDING       *)
+(* NEGLIGENCE OR OTHERWISE) ARISING IN ANY WAY OUT OF THE USE OF THIS         *)
+(* SOFTWARE, EVEN IF ADVISED OF THE POSSIBILITY OF SUCH DAMAGE.               *)
+(******************************************************************************)
+
+From Coq Require Import
+  Program.Equality.
+From Equations Require Import
+     Equations Signature.
+Require Import Equations.Prop.EqDec.
+
+From stdpp Require finite gmap list.
+
+From iris Require Import
+     algebra.auth
+     algebra.excl
+     algebra.gmap
+     base_logic.lib.fancy_updates
+     base_logic.lib.gen_heap
+     base_logic.lib.own
+     bi.big_op
+     bi.interface
+     program_logic.adequacy
+     program_logic.weakestpre
+     proofmode.tactics.
+
+From Katamaran Require Import
+     Iris.Base
+     Iris.Instance
+     Prelude
+     Semantics
+     Sep.Hoare
+     Sep.Logic
+     Signature
+     SmallStep.Step
+     Specification
+     BinaryResources.
+
+Import ctx.notations.
+Import env.notations.
+
+Set Implicit Arguments.
+
+(* The following three modules define the Iris instance of the program logic
+   depending solely on the operational semantics (through IrisBase) and the
+   user-defined predicates (in IrisPredicates), but without depending on a
+   Specification module. The program logic rules of this subset are implemented
+   in IrisSignatureRules, which is combined with IrisPredicates to form
+   IrisInstance.
+
+   This split allows us to use multiple different specifications with the same
+   Iris model, so that the resulting triples can be combined. This is important
+   particularly when combining specifications of universal contracts for unknown
+   code with known code verifications, e.g. as in the RiscvPmp.BlockVerification
+   proofs. *)
+
+Module Type IrisPredicates2
+  (Import B    : Base)
+  (Import SIG  : Signature B)
+  (Import PROG : Program B)
+  (Import SEM  : Semantics B PROG)
+  (Import IB   : IrisBase2 B PROG SEM).
+  Parameter luser_inst2 : forall `{sRG : sailRegGS2 Σ} `{invGS Σ} `{mG : memGS2 Σ} (p : 𝑯) (ts : Env Val (𝑯_Ty p)), iProp Σ.
+  Parameter lduplicate_inst2 : forall `{sRG : sailRegGS2 Σ} `{invGS Σ} {mG : memGS2 Σ} (p : 𝑯) (ts : Env Val (𝑯_Ty p)),
+      is_duplicable p = true ->
+      luser_inst2 ts ⊢ luser_inst2 ts ∗ luser_inst2 ts.
+
+End IrisPredicates2.
+
+Module IrisBinaryWP
+  (Import B     : Base)
+  (Import SIG   : Signature B)
+  (Import PROG  : Program B)
+  (Import SEM   : Semantics B PROG)
+  (Import IB2   : IrisBase2 B PROG SEM)
+  (Import IPred : IrisPredicates2 B SIG PROG SEM IB2).
+
+  Section WithSailGS2.
+    Context `{sG : sailGS2 Σ}.
+
+    #[export] Program Instance PredicateDefIProp : PredicateDef (iProp Σ) :=
+      {| lptsreg σ r v        := reg_pointsTo2 r v v;
+        luser p ts           := luser_inst2 ts;
+        lduplicate p ts Hdup := lduplicate_inst2 ts Hdup
+      |}.
+
+    (* Declare necessary OFE instances. Don't use them directly, they will be
+     resolved when needed. *)
+    Canonical Structure PCtxO     := leibnizO PCtx.
+    Canonical Structure TyO       := leibnizO Ty.
+    Canonical Structure CStoreO Γ := leibnizO (CStore Γ).
+    Canonical Structure StmO Γ τ  := leibnizO (Stm Γ τ).
+    Canonical Structure ValO τ    := leibnizO (Val τ).
+
+    Definition Post2 Γ1 Γ2 τ :=
+      Val τ -> CStore Γ1 -> Val τ -> CStore Γ2 -> iProp Σ.
+    Canonical Structure Post2O Γ1 Γ2 τ := leibnizO (Post2 Γ1 Γ2 τ).
+
+    Definition Wp2 Γ1 Γ2 τ :=
+      CStore Γ1 -d> CStore Γ2 -d>
+        Stm Γ1 τ -d> Stm Γ2 τ -d>
+        Post2 Γ1 Γ2 τ -d>
+        iProp Σ.
+
+    (* IDEA: borrow idea of Atomic of Iris. When s1 and s2 are atomic, they are
+           allowed to open the invariants and close them.
+           Some useful resources to look at:
+           - iris/program_logic/weakestpre.v > wp_atomic
+           - iris/program_logic/atomic.v > atomic_wp_inv
+
+           It might be that some restrictions that apply to wp2 are only
+           exposed at the ISA level (for example, MMIO interactions ≡ effects)
+
+           How does PMP come into play? Can we capture non-interferene of U-mode
+           data through invariants? (I would assume so)
+     *)
+    Ltac f_equiv_more_arities := match goal with
+                                 | H:_ ?f ?g |- ?R (?f ?x ?y ?z1) (?g ?x ?y ?z1) => solve [ simple apply H ]
+                                 | H:_ ?f ?g |- ?R (?f ?x ?y ?z1 ?z2) (?g ?x ?y ?z1 ?z2) => solve [ simple apply H ]
+                                 | H:_ ?f ?g |- ?R (?f ?x ?y ?z1 ?z2 ?z3) (?g ?x ?y ?z1 ?z2 ?z3) => solve [ simple apply H ]
+                                 end.
+
+    Ltac solve_contractive_more_arities := solve_proper_core ltac:(fun _ => first [ f_contractive | f_equiv | f_equiv_more_arities]).
+
+    Import SmallStepNotations.
+
+    Definition semWp2 {Γ1 Γ2 τ} : Wp2 Γ1 Γ2 τ :=
+      let sG_left    := sailGS2_sailGS_left in
+      let srGS_right := sailRegGS2_sailRegGS_right in
+      let mG_right   := memGS2_memGS_right in
+      (λ δ1 δ2 s1 s2 Q,
+        ∀ γ21 μ21,
+          regs_inv (srGS := srGS_right) γ21 ∗ mem_inv (mG := mG_right) μ21 -∗
+            semWP (sG := sG_left) s1 (λ v1 δ1',
+              ∃ γ22 μ22 δ2' v2,
+                ⌜⟨ γ21, μ21, δ2, s2 ⟩ --->* ⟨ γ22, μ22, δ2', stm_val τ v2 ⟩⌝
+                ∗ regs_inv (srGS := srGS_right) γ22 ∗ mem_inv (mG := mG_right) μ22
+                ∗ Q v1 δ1' v2 δ2'
+          ) δ1)%I.
+
+    Lemma semWp2_mono [Γ1 Γ2 τ] (s1 : Stm Γ1 τ) (s2 : Stm Γ2 τ)
+      (Q1 Q2 : Post2 Γ1 Γ2 τ) (δ1 : CStore Γ1) (δ2 : CStore Γ2) :
+      ⊢ semWp2 δ1 δ2 s1 s2 Q1 -∗ (∀ v1 δ1 v2 δ2, Q1 v1 δ1 v2 δ2 -∗ Q2 v1 δ1 v2 δ2) -∗ semWp2 δ1 δ2 s1 s2 Q2.
+    Admitted.
+
+    Lemma semWp2_val {Γ1 Γ2 τ} (v1 : Val τ) (v2 : Val τ) (Q : Post2 Γ1 Γ2 τ) :
+      forall δ1 δ2,
+        semWp2 δ1 δ2 (stm_val τ v1) (stm_val τ v2) Q ⊣⊢ |={⊤}=> Q v1 δ1 v2 δ2.
+    Admitted.
+
+    Lemma fupd_semWp2 {Γ1 Γ2 τ} E (δA : CStore Γ1) (δB : CStore Γ2)
+      (eA : Stm Γ1 τ) (eB : Stm Γ2 τ) Φ : 
+      (|={E}=> semWp2 δA δB eA eB Φ) ⊢ semWp2 δA δB eA eB Φ.
+    Admitted.
+
+    Lemma semWp2_step_fupd {Γ1 Γ2 τ} (δA : CStore Γ1) (δB : CStore Γ2)
+      (eA : Stm Γ1 τ) (eB : Stm Γ2 τ) (P :iProp Σ) Φ : 
+      to_val {| conf_stm := eA; conf_store := δA |} = None ->
+      to_val {| conf_stm := eB; conf_store := δB |} = None ->
+      P -∗
+           semWp2 δA δB eA eB (λ v1 δA v2 δB, P -∗ Φ v1 δA v2 δB) -∗
+                                                                     semWp2 δA δB eA eB Φ.
+    Admitted.
+
+    Lemma semWp2_frame_l {Γ1 Γ2 τ} (s1 : Stm Γ1 τ) (s2 : Stm Γ2 τ)
+      (δ1 : CStore Γ1) (δ2 : CStore Γ2) (POST : Post2 Γ1 Γ2 τ)
+      (R : iProp Σ) :
+      R ∗ semWp2 δ1 δ2 s1 s2 POST -∗
+                                     semWp2 δ1 δ2 s1 s2 (fun v1 δ1 v2 δ2 => R ∗ POST v1 δ1 v2 δ2).
+    Admitted.
+
+    Ltac discriminate_step :=
+      match goal with
+      | H: ⟨ ?γ, ?μ, ?δ, stm_fail ?τ ?m ⟩ ---> ⟨ ?γ', ?μ', ?δ', ?s ⟩ |- _ =>
+          inversion H
+      | H: ⟨ ?γ, ?μ, ?δ, stm_val ?τ ?v ⟩ ---> ⟨ ?γ', ?μ', ?δ', ?s ⟩ |- _ =>
+          inversion H
+      end.
+
+    Ltac close_later H :=
+      iMod (fupd_mask_subseteq empty) as H; first set_solver.
+
+    Ltac stm_val_fail_stuck :=
+      repeat match goal with
+        | H: ⟨ ?γ, ?μ, ?δ, ?s ⟩ ---> ⟨ ?γ', ?μ', ?δ', ?s' ⟩
+          |- context[stm_to_val ?s] => rewrite (stm_val_stuck H)
+        | H: ⟨ ?γ, ?μ, ?δ, ?s ⟩ ---> ⟨ ?γ', ?μ', ?δ', ?s' ⟩
+          |- context[stm_to_fail ?s] => rewrite (stm_fail_stuck H)
+        end.
+
+    Lemma semWp2_exp {Γ τ} (Φ : Post2 Γ Γ τ) eA eB δA δB :
+      Φ (eval eA δA) δA (eval eB δB) δB ⊢ semWp2 δA δB (stm_exp eA) (stm_exp eB) Φ.
+    Admitted.
+
+    (* TODO: move somewhere else? *)
+    Ltac semWp2_stuck_progress :=
+      repeat match goal with
+        | H: ⟨ ?γ1, ?μ1, ?δ1, ?s ⟩ ---> ⟨ ?γ2, ?μ2, ?δ2, ?s' ⟩
+          |- context[stm_to_val ?s] =>
+            rewrite (stm_val_stuck H)
+        | H: ⟨ ?γ1, ?μ1, ?δ1, ?s ⟩ ---> ⟨ ?γ2, ?μ2, ?δ2, ?s' ⟩
+          |- context[stm_to_fail ?s] =>
+            rewrite (stm_fail_stuck H)
+        end.
+
+    Lemma not_final_expanded : ∀ {Γ τ} (s : Stm Γ τ),
+        ~ Final s -> stm_to_val s = None ∧ stm_to_fail s = None.
+    Proof.
+      intros Γ τ s H; unfold Final in H; destruct s; auto; contradiction.
+    Qed.
+
+    Lemma stm_to_val_not_fail {Γ τ} {s : Stm Γ τ} :
+      forall {v}, stm_to_val s = Some v -> stm_to_fail s = None.
+    Proof. intros; by destruct s. Qed.
+
+    Lemma semWp2_bind {Γ τ σ} (s1 s2 : Stm Γ σ) (k1 k2 : Val σ → Stm Γ τ)
+      (Q : Post2 Γ Γ τ) (δ1 δ2 : CStore Γ) :
+      semWp2 δ1 δ2 s1 s2 (fun v1 δ12 v2 δ22 => semWp2 δ12 δ22 (k1 v1) (k2 v2) Q) ⊢
+        semWp2 δ1 δ2 (stm_bind s1 k1) (stm_bind s2 k2) Q.
+    Proof.
+    Admitted.
+
+    Lemma semWp2_block {Γ1 Γ2 τ Δ1 Δ2} (δΔ1 : CStore Δ1) (δΔ2 : CStore Δ2) (s1 : Stm (Γ1 ▻▻ Δ1) τ) (s2 : Stm (Γ2 ▻▻ Δ2) τ) :
+      ⊢ ∀ (Q : Val τ → CStore Γ1 → Val τ → CStore Γ2 → iProp Σ) (δ1 : CStore Γ1) (δ2 : CStore Γ2),
+          semWp2 (δ1 ►► δΔ1) (δ2 ►► δΔ2) s1 s2 (fun v1 δ21 v2 δ22 => Q v1 (env.drop Δ1 δ21) v2 (env.drop Δ2 δ22)) -∗
+                                                                                                                     semWp2 δ1 δ2 (stm_block δΔ1 s1) (stm_block δΔ2 s2) Q.
+    Proof.
+    Admitted.
+
+    Lemma semWp2_let {Γ τ x σ} (s1 s2 : Stm Γ σ) (k1 k2 : Stm (Γ ▻ x∷σ) τ)
+      (Q : Post2 Γ Γ τ) (δ1 δ2 : CStore Γ) :
+      ⊢ semWp2 δ1 δ2 s1 s2 (fun v1 δ12 v2 δ22 => semWp2 δ12.[x∷σ ↦ v1] δ22.[x∷σ ↦ v2] k1 k2 (fun v12 δ13 v22 δ23 => Q v12 (env.tail δ13) v22 (env.tail δ23)) ) -∗
+                                                                                                                                                                  semWp2 δ1 δ2 (let: x ∷ σ := s1 in k1)%exp (let: x ∷ σ := s2 in k2)%exp Q.
+    Proof.
+    Admitted.
+
+    Lemma semWp2_seq {Γ τ σ} (s1 s2 : Stm Γ σ) (k1 k2 : Stm Γ τ) :
+      ⊢ ∀ (Q : Post2 Γ Γ τ) (δ1 δ2 : CStore Γ),
+          semWp2 δ1 δ2 s1 s2 (fun v1 δ21 v2 δ22 => semWp2 δ21 δ22 k1 k2 Q) -∗ semWp2 δ1 δ2 (s1;;k1)%exp (s2;;k2)%exp Q.
+    Proof.
+    Admitted.
+
+    Lemma semWp2_assertk {Γ τ} (e11 e21 : Exp Γ ty.bool) (e12 e22 : Exp Γ ty.string) (k1 k2 : Stm Γ τ) :
+      ⊢ ∀ (Q : Val τ → CStore Γ → Val τ → CStore Γ → iProp Σ) (δ1 δ2 : CStore Γ),
+          ⌜eval e11 δ1 = eval e21 δ2⌝ -∗
+                                         (⌜eval e11 δ1 = true⌝ → ⌜eval e21 δ2 = true⌝ → semWp2 δ1 δ2 k1 k2 Q) -∗
+                                                                                                                 semWp2 δ1 δ2 (stm_assertk e11 e12 k1) (stm_assertk e21 e22 k2) Q.
+    Proof.
+    Admitted.
+
+    Lemma semWp2_read_register {Γ τ} (reg : 𝑹𝑬𝑮 τ) :
+      ⊢ ∀ (Q : Val τ → CStore Γ → Val τ → CStore Γ → iProp Σ) (δ1 δ2 : CStore Γ),
+          (∃ v1 v2 : Val τ, reg_pointsTo2 reg v1 v2 ∗ (reg_pointsTo2 reg v1 v2 -∗ Q v1 δ1 v2 δ2)) -∗
+                                                                                                     semWp2 δ1 δ2 (stm_read_register reg) (stm_read_register reg) Q.
+    Proof.
+    Admitted.
+
+    Lemma semWp2_write_register {Γ τ} (reg : 𝑹𝑬𝑮 τ) (e1 e2 : Exp Γ τ) :
+      ⊢ ∀ (Q : Val τ → CStore Γ → Val τ → CStore Γ → iProp Σ) (δ1 δ2 : CStore Γ),
+          (∃ v1 v2 : Val τ, reg_pointsTo2 reg v1 v2 ∗ (reg_pointsTo2 reg (eval e1 δ1) (eval e2 δ2) -∗ Q (eval e1 δ1) δ1 (eval e2 δ2) δ2)) -∗
+                                                                                                                                             semWp2 δ1 δ2 (stm_write_register reg e1) (stm_write_register reg e2) Q.
+    Proof.
+    Admitted.
+
+    (* TODO: notation for cstore update not working? (import env.notations doesn't solve it) Investigate and define lemma *)
+    (* Lemma semWp2_assign {Γ τ x} (xInΓ : x∷τ ∈ Γ) (s1 s2 : Stm Γ τ) : *)
+    (*   ⊢ ∀ (Q : Val τ → CStore Γ → Val τ → CStore Γ → iProp Σ) (δ1 δ2 : CStore Γ), *)
+    (*       semWp2 δ1 δ2 s1 s2 (λ v1 δ21 v2 δ22, Q v1 (δ21 ⟪ x ↦ v1 ⟫) v2 (δ22 ⟪ x ↦ v2 ⟫)) -∗ *)
+    (*       semWp2 δ1 δ2 (stm_assign x s1) (stm_assign x s2) Q. *)
+    (* Proof. *)
+    (* Admitted. *)
+
+    Lemma semWp2_pattern_match {Γ τ σ} (s1 s2 : Stm Γ σ) (pat : Pattern σ)
+      (rhs1 rhs2 : ∀ pc : PatternCase pat, Stm (Γ ▻▻ PatternCaseCtx pc) τ) :
+      ⊢ ∀ (Q : Val τ → CStore Γ → Val τ → CStore Γ → iProp Σ) (δ1 δ2 : CStore Γ),
+          semWp2 δ1 δ2 s1 s2
+            (fun vσ1 δ12 vσ2 δ22 =>
+               let (pc1,δpc1) := pattern_match_val pat vσ1 in
+               let (pc2,δpc2) := pattern_match_val pat vσ2 in
+               semWp2 (δ12 ►► δpc1) (δ22 ►► δpc2) (rhs1 pc1) (rhs2 pc2)
+                 (fun vτ1 δ21 vτ2 δ22 => Q vτ1 (env.drop (PatternCaseCtx pc1) δ21) vτ2 (env.drop (PatternCaseCtx pc2) δ22))
+            ) -∗
+                 semWp2 δ1 δ2 (stm_pattern_match s1 pat rhs1) (stm_pattern_match s2 pat rhs2) Q.
+    Proof.
+    Admitted.
+
+    Lemma semWp2_foreign {Γ Δ τ} {f1 f2 : 𝑭𝑿 Δ τ} {es1 es2 : NamedEnv (Exp Γ) Δ} {Q δ1 δ2} :
+      ⊢ (∀ γ1 γ2 μ1 μ2,
+            (regs_inv2 γ1 γ2 ∗ mem_inv2 μ1 μ2)
+            ={⊤,∅}=∗
+                     (∀ res1 γ1' μ1' res2 γ2' μ2',
+                         ⌜ ForeignCall f1 (evals es1 δ1) res1 γ1 γ1' μ1 μ1' ⌝
+                           ∗ ⌜ ForeignCall f2 (evals es2 δ2) res2 γ2 γ2' μ2 μ2' ⌝
+                         ={∅}▷=∗
+                                 |={∅,⊤}=>
+                        (regs_inv2 γ1' γ2' ∗ mem_inv2 μ1' μ2') ∗
+                          semWp2 δ1 δ2 (match res1 with inr v => stm_val _ v
+                                                   | inl s => stm_fail _ s
+                                        end)
+                          (match res2 with inr v => stm_val _ v
+                                      | inl s => stm_fail _ s
+                           end)
+                          Q)) -∗
+                                 semWp2 δ1 δ2 (stm_foreign f1 es1) (stm_foreign f2 es2) Q.
+    Proof.
+    Admitted.
+
+    Lemma semWp2_debugk {Γ τ} (s1 s2 : Stm Γ τ) :
+      ⊢ ∀ Q δ1 δ2, semWp2 δ1 δ2 s1 s2 Q -∗ semWp2 δ1 δ2 (stm_debugk s1) (stm_debugk s2) Q.
+    Proof.
+    Admitted.
+
+    Lemma semWp2_lemmak {Γ τ} {Δ} (l1 l2 : 𝑳 Δ) (es1 es2 : NamedEnv (Exp Γ) Δ) (s1 s2 : Stm Γ τ) :
+      ⊢ ∀ Q δ1 δ2, semWp2 δ1 δ2 s1 s2 Q -∗ semWp2 δ1 δ2 (stm_lemmak l1 es1 s1) (stm_lemmak l2 es2 s2) Q.
+    Proof.
+    Admitted.
+  End WithSailGS2.
+End IrisBinaryWP.
+
+Module Type IrisSignatureRules2
+  (Import B     : Base)
+  (Import SIG   : Signature B)
+  (Import PROG  : Program B)
+  (Import SEM   : Semantics B PROG)
+  (Import IB2   : IrisBase2 B PROG SEM)
+  (Import IPred : IrisPredicates2 B SIG PROG SEM IB2).
+
+  Module Export IWP := IrisBinaryWP B SIG PROG SEM IB2 IPred.
+
+  Section WithSailGS2.
+  Context `{sG : sailGS2 Σ}.
+
+Section Soundness.
+
+  Definition semTriple {Γ τ} (δ : CStore Γ)
+             (PRE : iProp Σ) (s : Stm Γ τ) (POST : Val τ -> CStore Γ -> iProp Σ) : iProp Σ :=
+    PRE -∗
+           semWp2 δ δ s s (fun v1 δ1 v2 δ2 => ⌜ v1 = v2 ⌝ ∗ ⌜ δ1 = δ2 ⌝ ∗ POST v1 δ1)%I.
+  (* always modality needed? perhaps not because sail not higher-order? *)
+  Global Arguments semTriple {Γ} {τ} δ PRE%I s%exp POST%I.
+
+  Definition ValidLemma {Δ} (lem : Lemma Δ) : Prop :=
+    match lem with
+      {| lemma_logic_variables := Σ;
+         lemma_patterns        := θΔ;
+         lemma_precondition    := req;
+         lemma_postcondition   := ens;
+      |} =>
+      forall (ι : Valuation Σ),
+        ⊢ asn.interpret req ι -∗
+          asn.interpret ens ι
+    end.
+
+  Lemma iris_rule_consequence {Γ σ} {δ : CStore Γ}
+        {P P'} {Q Q' : Val σ -> CStore Γ -> iProp Σ} {s : Stm Γ σ} :
+        (P ⊢ P') -> (forall v δ', Q' v δ' ⊢ Q v δ') ->
+        semTriple δ P' s Q' -∗ semTriple δ P s Q.
+  Proof.
+    iIntros (PP QQ) "Htriple P".
+    iApply (semWp2_mono with "[Htriple P]").
+    - iApply "Htriple".
+      now iApply PP.
+    - iIntros (v1 δ1 v2 δ2) "(-> & -> & Q')".
+      iPoseProof (QQ with "Q'") as "Q"; auto.
+  Qed.
+
+  Lemma iris_rule_frame {Γ σ} {δ : CStore Γ}
+        (R P : iProp Σ) (Q : Val σ -> CStore Γ -> iProp Σ) (s : Stm Γ σ) :
+        (⊢ semTriple δ P s Q -∗ semTriple δ (R ∗ P) s (fun v δ' => R ∗ Q v δ'))%I.
+  Proof.
+    iIntros "Htriple [HR HP]".
+    iSpecialize ("Htriple" with "HP").
+    iPoseProof (semWp2_frame_l with "[HR Htriple]") as "Hwp".
+    { iSplitL "HR". iExact "HR". iExact "Htriple". }
+    iApply (semWp2_mono with "Hwp").
+    iIntros (? ? ? ?) "($ & $ & $ & $)".
+  Qed.
+
+  Lemma iris_rule_pull {σ Γ} (δ : CStore Γ) (s : Stm Γ σ)
+        (P : iProp Σ) (Q : Prop) (R : Val σ -> CStore Γ -> iProp Σ) :
+        (⊢ (⌜ Q ⌝ → semTriple δ P s R) -∗ semTriple δ (P ∧ bi_pure Q) s R).
+  Proof.
+    iIntros "QP [P %]".
+    by iApply "QP".
+  Qed.
+
+  Lemma iris_rule_exist {σ Γ} (δ : CStore Γ)
+        (s : Stm Γ σ) {A : Type} {P : A -> iProp Σ}
+        {Q :  Val σ -> CStore Γ -> iProp Σ} :
+        ⊢ ((∀ x, semTriple δ (P x) s Q) -∗ semTriple δ (∃ x, P x) s Q).
+  Proof.
+    iIntros "Htriple [% P]".
+    by iApply "Htriple".
+  Qed.
+
+  Lemma iris_rule_stm_val {Γ} (δ : CStore Γ)
+        {τ : Ty} {v : Val τ}
+        {P : iProp Σ} {Q : Val τ -> CStore Γ -> iProp Σ} :
+        ⊢ ((P -∗ Q v δ)%I -∗ semTriple δ P (stm_val τ v) Q).
+  Proof.
+    iIntros "PQ P".
+    iApply semWp2_val.
+    iSpecialize ("PQ" with "P").
+    iModIntro; by iFrame.
+  Qed.
+
+  Lemma iris_rule_stm_exp {Γ} (δ : CStore Γ)
+        {τ : Ty} {e : Exp Γ τ}
+        {P : iProp Σ} {Q : Val τ -> CStore Γ -> iProp Σ} :
+        ⊢ ((P -∗ Q (eval e δ) δ) -∗ semTriple δ P (stm_exp e) Q).
+  Proof.
+    iIntros "PQ P".
+    iApply semWp2_exp.
+    iSpecialize ("PQ" with "P").
+    now iFrame.
+  Qed.
+
+  Lemma iris_rule_stm_let {Γ} (δ : CStore Γ)
+        (x : PVar) (σ τ : Ty) (s : Stm Γ σ) (k : Stm (Γ ▻ x∷σ) τ)
+        (P : iProp Σ) (Q : Val σ -> CStore Γ -> iProp Σ)
+        (R : Val τ -> CStore Γ -> iProp Σ) :
+        ⊢ (semTriple δ P s Q -∗
+                     (∀ (v : Val σ) (δ' : CStore Γ),
+                         semTriple (env.snoc δ' (x∷σ) v) (Q v δ') k (fun v δ'' => R v (env.tail δ'')) ) -∗
+                     semTriple δ P (let: x := s in k) R).
+  Proof.
+    iIntros "Hs Hk P".
+    iApply semWp2_let.
+    iSpecialize ("Hs" with "P").
+    iApply (semWp2_mono with "Hs").
+    iIntros (v1 δ1 v2 δ2) "(<- & <- & Q)".
+    iSpecialize ("Hk" $! v1 δ1 with "Q").
+    iApply (semWp2_mono with "Hk").
+    iIntros (? ? ? ?) "(<- & <- & R)".
+    by iFrame"R".
+  Qed.
+
+  Lemma iris_rule_stm_block {Γ} (δ : CStore Γ)
+        (Δ : PCtx) (δΔ : CStore Δ)
+        (τ : Ty) (k : Stm (Γ ▻▻ Δ) τ)
+        (P : iProp Σ) (R : Val τ -> CStore Γ -> iProp Σ) :
+        ⊢ (semTriple (δ ►► δΔ) P k (fun v δ'' => R v (env.drop Δ δ'')) -∗
+                   semTriple δ P (stm_block δΔ k) R).
+  Proof.
+  Admitted.
+
+  Lemma iris_rule_stm_seq {Γ} (δ : CStore Γ)
+        (τ : Ty) (s1 : Stm Γ τ) (σ : Ty) (s2 : Stm Γ σ)
+        (P : iProp Σ) (Q : CStore Γ -> iProp Σ) (R : Val σ -> CStore Γ -> iProp Σ) :
+    ⊢ (semTriple δ P s1 (fun _ => Q) -∗
+                 (∀ δ', semTriple δ' (Q δ') s2 R) -∗
+                 semTriple δ P (s1 ;; s2) R).
+  Proof.
+  Admitted.
+
+  Lemma iris_rule_stm_assertk {Γ τ} (δ : CStore Γ)
+        (e1 : Exp Γ ty.bool) (e2 : Exp Γ ty.string) (k : Stm Γ τ)
+                      (P : iProp Σ) (Q : Val τ -> CStore Γ -> iProp Σ) :
+    ⊢ (⌜ eval e1 δ = true ⌝ → semTriple δ P k Q) -∗
+      semTriple δ P (stm_assertk e1 e2 k) Q.
+  Proof.
+  Admitted.
+
+  Lemma iris_rule_stm_fail {Γ} (δ : CStore Γ)
+        (τ : Ty) (s : Val ty.string) :
+        forall (Q : Val τ -> CStore Γ -> iProp Σ),
+          ⊢ semTriple δ True (stm_fail τ s) Q.
+  Proof.
+  Admitted.
+
+  Lemma iris_rule_stm_read_register {Γ} (δ : CStore Γ)
+        {σ : Ty} (r : 𝑹𝑬𝑮 σ) (v : Val σ) :
+        ⊢ (semTriple δ (lptsreg r v) (stm_read_register r) (fun v' δ' => ⌜ δ' = δ ⌝ ∧ ⌜ v' = v ⌝ ∧ lptsreg r v)).
+  Proof.
+  Admitted.
+
+  Lemma iris_rule_stm_write_register {Γ} (δ : CStore Γ)
+        {σ : Ty} (r : 𝑹𝑬𝑮 σ) (w : Exp Γ σ)
+                              (Q : Val σ -> CStore Γ -> iProp Σ)
+                              (v : Val σ) :
+        ⊢ semTriple δ (lptsreg r v) (stm_write_register r w)
+                  (fun v' δ' => ⌜δ' = δ⌝ ∧ ⌜v' = eval w δ⌝ ∧ lptsreg r v').
+  Proof.
+  Admitted.
+
+  Lemma iris_rule_stm_assign {Γ} (δ : CStore Γ)
+        (x : PVar) (σ : Ty) (xIn : x∷σ ∈ Γ) (s : Stm Γ σ)
+        (P : iProp Σ) (R : Val σ -> CStore Γ -> iProp Σ) :
+        ⊢ (semTriple δ P s (fun v δ' => R v (@env.update _ _ _ δ' (x∷_) _ v)) -∗
+           semTriple δ P (stm_assign x s) R).
+  Proof.
+  Admitted.
+
+  Lemma iris_rule_stm_bind {Γ} (δ : CStore Γ)
+        {σ τ : Ty} (s : Stm Γ σ) (k : Val σ -> Stm Γ τ)
+        (P : iProp Σ) (Q : Val σ -> CStore Γ -> iProp Σ)
+        (R : Val τ -> CStore Γ -> iProp Σ) :
+        ⊢ (semTriple δ P s Q -∗
+           (∀ (v__σ : Val σ) (δ' : CStore Γ),
+               semTriple δ' (Q v__σ δ') (k v__σ) R) -∗
+           semTriple δ P (stm_bind s k) R).
+  Proof.
+    iIntros "trips tripk P".
+    iSpecialize ("trips" with "P").
+    iApply semWp2_bind.
+    iApply (semWp2_mono with "trips").
+    iIntros (v1 δ1 v2 δ2) "(<- & <- & HR)".
+    now iApply ("tripk" with "HR").
+  Qed.
+
+  Lemma iris_rule_stm_call_inline_later
+    {Γ} (δΓ : CStore Γ)
+    {Δ σ} (f : 𝑭 Δ σ) (es : NamedEnv (Exp Γ) Δ)
+    (P : iProp Σ) (Q : Val σ -> CStore Γ -> iProp Σ) :
+    ⊢ ▷ semTriple (evals es δΓ) P (FunDef f) (fun v _ => Q v δΓ) -∗
+      semTriple δΓ P (stm_call f es) Q.
+  Proof.
+  Admitted.
+
+  Lemma iris_rule_stm_call_inline
+    {Γ} (δΓ : CStore Γ)
+    {Δ σ} (f : 𝑭 Δ σ) (es : NamedEnv (Exp Γ) Δ)
+    (P : iProp Σ) (Q : Val σ -> CStore Γ -> iProp Σ) :
+    ⊢ semTriple (evals es δΓ) P (FunDef f) (fun v _ => Q v δΓ) -∗
+      semTriple δΓ P (stm_call f es) Q.
+  Proof.
+  Admitted.
+
+  Lemma iris_rule_stm_debugk
+    {Γ τ} (δ : CStore Γ) (k : Stm Γ τ)
+    (P : iProp Σ) (Q : Val τ -> CStore Γ -> iProp Σ) :
+    ⊢ (semTriple δ P k Q -∗
+       semTriple δ P (stm_debugk k) Q).
+  Proof.
+  Admitted.
+
+  Lemma iris_rule_noop {Γ σ} {δ : CStore Γ}
+        {P} {Q : Val σ -> CStore Γ -> iProp Σ} {s : Stm Γ σ} :
+    stm_to_val s = None ->
+    stm_to_fail s = None ->
+    (forall {s' γ γ' μ μ' δ'}, ⟨ γ, μ, δ, s ⟩ ---> ⟨ γ', μ', δ', s' ⟩ ->
+                            (γ' = γ) /\ (μ' = μ) /\ (δ' = δ) /\
+                              (forall {s2 : Stm Γ σ} {γ2 μ2} {δ2 : CStore Γ}, ⟨ γ2, μ2, δ2, s2 ⟩ ---> ⟨ γ2, μ2, δ2, s' ⟩) /\
+                            ((exists v, s' = stm_val _ v) \/ (exists msg, s' = stm_fail _ msg))) ->
+    (∀ v, P ={⊤}=∗ Q v δ) -∗
+                 semTriple δ P s Q.
+  Proof.
+  Admitted.
+
+  Lemma iris_rule_stm_pattern_match {Γ τ σ} (δΓ : CStore Γ)
+    (s : Stm Γ σ) (pat : Pattern σ)
+    (rhs : ∀ pc : PatternCase pat, Stm (Γ ▻▻ PatternCaseCtx pc) τ)
+    (P : iProp Σ) (Q : Val σ → CStore Γ → iProp Σ) (R : Val τ → CStore Γ → iProp Σ) :
+    ⊢ semTriple δΓ P s Q -∗
+      (∀ pc δpc δΓ1,
+         semTriple (δΓ1 ►► δpc) (Q (pattern_match_val_reverse pat pc δpc) δΓ1) (rhs pc)
+           (λ vτ (δ' : CStore (Γ ▻▻ PatternCaseCtx pc)), R vτ (env.drop (PatternCaseCtx pc) δ'))) -∗
+      semTriple δΓ P (stm_pattern_match s pat rhs) R.
+  Proof.
+  Admitted.
+
+  Definition ValidContractSemCurried {Δ σ} (body : Stm Δ σ) (contract : SepContract Δ σ) : iProp Σ :=
+    match contract with
+    | MkSepContract _ _ ctxΣ θΔ pre result post =>
+      Sep.Logic.Forall (fun (ι : Valuation ctxΣ) =>
+        semTriple (inst θΔ ι) (asn.interpret pre ι) body
+                  (fun v δ' => asn.interpret post (env.snoc ι (result∷σ) v)))
+    end.
+
+  Definition ValidContractSem {Δ σ} (body : Stm Δ σ) (contract : SepContract Δ σ) : iProp Σ :=
+    match contract with
+    | MkSepContract _ _ ctxΣ θΔ pre result post =>
+      ∀ (ι : Valuation ctxΣ),
+        semTriple (inst θΔ ι) (asn.interpret pre ι) body
+                  (fun v δ' => asn.interpret post (env.snoc ι (result∷σ) v))
+    end.
+
+  Definition ValidContractForeign {Δ τ} (contract : SepContract Δ τ) (f : 𝑭𝑿 Δ τ) : Prop :=
+    forall Γ (es : NamedEnv (Exp Γ) Δ) (δ : CStore Γ),
+      match contract with
+      | MkSepContract _ _ Σ' θΔ req result ens =>
+        forall (ι : Valuation Σ'),
+        evals es δ = inst θΔ ι ->
+        ⊢ semTriple δ (asn.interpret req ι) (stm_foreign f es)
+          (fun v δ' => asn.interpret ens (env.snoc ι (result∷τ) v) ∗ bi_pure (δ' = δ))
+      end.
+
+  Definition valid_contract_curry {Δ σ} (body : Stm Δ σ) (contract : SepContract Δ σ) :
+    ValidContractSem body contract ⊣⊢ ValidContractSemCurried body contract.
+  Proof.
+    destruct contract as [lvars δ req res ens]; cbn.
+    now rewrite Forall_forall.
+  Qed.
+
+End Soundness.
+End WithSailGS2.
+
+End IrisSignatureRules2.
